Major rewrite.... needs refactor

src/geom/basic.lean
@@ -1,9 +1,0 @@
-import ..pregeom.basic
-
-variable (T : Type*)
-
-class inf_geom extends inf_reg_pregeom T :=
-(cl_singleton {x} : cl {x} = {x})
-
-class geom extends reg_pregeom T :=
-(cl_singleton {x} : cl {x} = {x})
