src/pregeom/basic.lean
@@ -1,114 +1,132 @@
-import data.finset
+import data.set
 
-open_locale classical
+class has_cl (T : Type*) := (cl : set T → set T)
 
-variable (T : Type*)
-
-class has_cl :=
-(cl : set T → set T)
-
-open has_cl
-open has_insert
-
-class inf_pregeom extends has_cl T :=
-(inclusive {S} : S ⊆ cl S)
-(monotone {S1 S2} : S1 ⊆ S2 → cl S1 ⊆ cl S2)
+class pregeom (T : Type*) extends has_cl T :=
+(inclusive {S} : S ≤ cl S)
+(monotone {A B} : A ≤ B → cl A ≤ cl B)
 (idempotent {S} : cl (cl S) = cl S)
-(exchange {x y} {S} : x ∈ cl (insert y S) → x ∉ cl S → y ∈ cl (insert x S))
+(exchange {x y S} : x ∈ cl (insert y S) → x ∉ cl S → y ∈ cl (insert x S))
+(finchar {x S} : x ∈ cl S → ∃ A : finset T, ↑A ≤ S ∧ x ∈ cl ↑A)
 
-class inf_reg_pregeom extends inf_pregeom T :=
-(regular : cl ∅ = ∅)
+class geometry (T : Type*) extends pregeom T :=
+(cl_singleton {x} : cl {x} = {x})
+(cl_empty : cl ∅ = ∅)
 
-class pregeom extends inf_pregeom T := 
-(finchar {x} {S} : x ∈ cl S → ∃ U : finset T, ↑U ⊆ S ∧ x ∈ cl ↑U)
+namespace pregeom
+open has_cl
 
-class reg_pregeom extends pregeom T :=
-(regular : cl ∅ = ∅)
+variables {T : Type*} 
 
-namespace has_cl
+def is_closed [has_cl T] (S : set T) := ∃ A, cl A = S 
+def cls [has_cl T] (x : T) := cl ({x} : set T)
 
-lemma reg_set_incl [has_cl T] {S : set T} : {t : T | t ∉ cl (∅ : set T)} ∩ S ⊆ S := by exact {t : T | t ∉ cl ∅}.inter_subset_right S
-
-end has_cl
-
-namespace inf_pregeom 
-variable [inf_pregeom T]
-variable {T}
-
-lemma mem_cl_of_subset_mem {x : T} {A B : set T} : A ⊆ B → x ∈ cl A → x ∈ cl B := 
-begin
-  intros h hx,
-  exact inf_pregeom.monotone h hx,
-end
-
-lemma cl_union_cl_subset_cl_union {A B : set T} : cl A ∪ cl B ⊆ cl (A ∪ B) :=
-begin
-  intros s hs,
-  cases hs,
-  {
-    have : A ⊆ A ∪ B, by exact set.subset_union_left A B,
-    exact monotone this hs,
-  },
-  {
-    have : B ⊆ A ∪ B, by exact set.subset_union_right A B,
-    exact monotone this hs,
-  },
-end
+lemma mem_cls [pregeom T] {x : T} : x ∈ cls x := inclusive (set.mem_singleton x)
 
 @[simp]
-lemma cl_cl_union {A B : set T} : cl (cl A ∪ B) = cl (A ∪ B) := 
+lemma cls_le [pregeom T] {x : T} {S : set T} : cls x ≤ cl S ↔ x ∈ cl S := 
 begin
-  ext,
   split,
   {
-    intro h,
-    rw ←idempotent,
-    have : cl A ∪ B ⊆ cl (A ∪ B),
-    {
-      intros t ht,
-      cases ht,
-      {
-        have : A ⊆ A ∪ B, by exact set.subset_union_left A B,
-        replace this := monotone this,
-        apply this,
-        assumption,
-      },
-      {
-        have : B ⊆ A ∪ B, by exact set.subset_union_right A B,
-        replace this := monotone this,
-        apply this, apply inclusive, assumption,
-      }
-    },
-    replace this := monotone this,
-    apply this,
-    assumption,
+    intro hx,
+    apply hx, 
+    exact mem_cls,
   },
   {
-    have : A ∪ B ⊆ cl A ∪ B, by exact set.union_subset_union_left B inclusive,
-    intro h,
-    exact monotone this h,
+    intro hx,
+    suffices : cls x ≤ cl (cl S), by rwa idempotent at this,
+    apply monotone, 
+    rintros y ⟨rfl⟩, 
+    assumption,
   }
 end
 
 @[simp]
-lemma cl_union_cl {A B : set T} : cl (A ∪ cl B) = cl (A ∪ B) := 
+lemma Sup_all_le_cl [pregeom T] {S : set T} : Sup { A | ∃ x, A = cls x ∧ A ≤ cl S } = cl S :=
 begin
-  have : A ∪ cl B = cl B ∪ A, by exact sup_comm, rw this,
-  have : A ∪ B = B ∪ A, by exact sup_comm, rw this,
-  exact cl_cl_union
+  ext, split,
+  {
+    intro hx,
+    rcases hx with ⟨A, ⟨t,rfl,h⟩, hA⟩,
+    exact h hA,
+  },
+  {
+    intro hx,
+    refine ⟨cls x, ⟨x,rfl, _⟩,_⟩,
+    { rw cls_le, exact hx },
+    { exact mem_cls },
+  }
 end
 
-@[simp]
-lemma cl_cl_union_cl {A B : set T} : cl (cl A ∪ cl B) = cl (A ∪ B) := 
+lemma exchange_cls [pregeom T] {u v : T} (h1 : u ∈ cls v) (h2 : u ∉ cl (∅ : set T))  : v ∈ cls u :=
+begin
+  unfold cls at *,
+  rw set.singleton_def at *,
+  exact exchange h1 h2,
+end
+
+lemma cls_le_of_mem [pregeom T] {x : T} {S : set T} : x ∈ cl S ↔ cls x ≤ cl S := 
+begin
+  split; intro hx,
+  {
+    have : ({x} : set T) ≤ cl S, 
+    {
+      rintros y ⟨hy⟩,
+      assumption,
+    },
+    replace this := monotone this,
+    rw idempotent at this,
+    assumption,
+  },
+  {
+    apply hx,
+    exact mem_cls,
+  }
+end
+
+lemma cl_cl_union [pregeom T] {A B : set T} : cl (cl A ∪ B) = cl (A ∪ B) := 
+begin
+  ext, split; intro h,
+  {
+    rw ←idempotent,
+    refine monotone _ h,
+    intros y hy,
+    cases hy,
+    {
+      refine monotone _ hy,
+      intros a ha,
+      left, assumption,
+    },
+    {
+      apply inclusive,
+      right, assumption,
+    }
+  },
+  {
+    refine monotone _ h,
+    intros z hz,
+    cases hz,
+    {
+      left,
+      apply inclusive, assumption,
+    },
+    {
+      right, assumption,
+    }
+  }
+end
+
+lemma cl_union_cl [pregeom T] {A B : set T} : cl (A ∪ cl B) = cl (A ∪ B) := 
+calc cl (A ∪ cl B) = cl (A ⊔ cl B) : rfl
+... = cl (cl B ⊔ A) : by rw sup_comm
+... = cl (cl B ∪ A) : rfl
+... = cl (B ∪ A) : cl_cl_union
+... = cl (B ⊔ A) : rfl
+... = cl (A ⊔ B) : by rw sup_comm
+... = cl (A ∪ B) : rfl
+
+lemma cl_cl_union_cl [pregeom T] {A B : set T} : cl (cl A ∪ cl B) = cl (A ∪ B) := 
 calc cl (cl A ∪ cl B) = cl (cl A ∪ B) : cl_union_cl
 ... = cl (A ∪ B) : cl_cl_union
 
-@[simp]
-lemma cl_empty_union [inf_pregeom T] {S : set T} :
-  cl (cl (∅ : set T) ∪ S) = cl S := 
-calc cl (cl (∅ : set T) ∪ S) = cl (cl ∅ ∪ cl S) : by rw ←cl_union_cl
-... = cl (∅ ∪ cl S) : by rw cl_cl_union
-... = cl (cl S) : by rw set.empty_union
-... = cl S : by rw inf_pregeom.idempotent
-
-end inf_pregeom
+end pregeom
