src/pregeom/geometrize.lean
@@ -1,0 +1,490 @@
+import .basic
+import ..subtype.helpers
+import data.finset
+
+open_locale classical
+
+namespace pregeom
+open has_cl
+
+variables (T : Type*) 
+
+def reg_set [has_cl T] := { t | t ∉ cl (∅ : set T) }
+def reg [has_cl T] := subtype (reg_set T)
+
+namespace reg
+
+local notation `ι` := subtype.val
+
+instance has_cl_instance [has_cl T] : has_cl (reg T) :=
+⟨ λ S, ι ⁻¹' cl (ι '' S) ⟩
+
+protected def rel [has_cl T] : reg T → reg T → Prop :=
+λ s t, cls s = cls t 
+
+variable {T}
+
+protected theorem is_equiv [has_cl T] : equivalence (reg.rel T) := 
+begin
+  refine ⟨_,_,_⟩,
+  {
+    unfold reflexive reg.rel,
+    intro x, refl,
+  },
+  {
+    unfold symmetric reg.rel,
+    rintros x y hx,
+    rwa hx,
+  },
+  {
+    unfold transitive reg.rel,
+    intros x y z h1 h2,
+    rwa [h1,h2],
+  }
+end
+
+@[simp]
+lemma cl_union_cl_empty [pregeom T] {A : set T} : cl (cl (∅ : set T) ∪ A) = cl A := 
+begin
+  rw [←pregeom.cl_cl_union_cl, idempotent],
+  have : cl ∅ ≤ cl A, 
+  {
+    refine monotone _, 
+    tauto,
+  },
+  replace this : cl (∅ : set T) ∪ cl A = cl A,
+  {
+    ext, split; intro h,
+    { cases h, { apply this, assumption }, { assumption }},
+    { right, assumption }
+  },
+  rw [this, idempotent],
+end
+
+@[simp]
+lemma cl_reg_set_inter [pregeom T] {S : set T} : cl (reg_set T ∩ S) = cl S := 
+begin
+  ext, split,
+  {
+    intro h,
+    have : reg_set T ∩ S ≤ S, by {intros x hx, cases hx, assumption},
+    exact monotone this h,
+  },
+  {
+    intro h,
+    have : S ≤ cl (∅ : set T) ∪ (reg_set T ∩ S), 
+    {
+      intros s hs,
+      by_cases s ∈ cl (∅ : set T),
+      { left, assumption },
+      {
+        right,
+        exact ⟨h,hs⟩,
+      }
+    },
+    replace h := monotone this h,
+    rw cl_union_cl_empty at h,
+    exact h,
+  }
+end
+
+
+private lemma reg_lift_finset [has_cl T] {W : finset T} : ↑W ⊆ reg_set T → ∃ V : finset (reg T), finset.image ι V = W := 
+begin
+  refine finset.induction_on W _ _; intros,
+  {
+    use ∅,
+    trivial,
+  },
+  {
+    have : ↑s ⊆ reg_set T,
+    {
+      intros x hx,
+      apply a_3,
+      simp [hx],
+    },
+    rcases a_2 this with ⟨V,rfl⟩,
+    have : a ∈ reg_set T,
+    {
+      apply a_3,
+      simp,
+    },
+    use insert ⟨a,this⟩ V,
+    rwa finset.image_insert,
+  }
+end
+
+instance pregeom_instance [pregeom T] : pregeom (reg T) :=
+begin
+  split; intros,
+  {
+    intros s hs,
+    change s.val ∈ _,
+    apply inclusive,
+    exact set.mem_image_of_mem ι hs,
+  },
+  {
+    -- this needs some cleaning up...
+    intros u hu,
+    change u.val ∈ cl (ι '' B),
+    suffices : ι '' A ≤ ι '' B, by exact monotone this hu,
+    intros x hx,
+    rcases hx with ⟨y,h,rfl⟩,
+    suffices : y ∈ B, by exact set.mem_image_of_mem ι this,
+    exact a h,
+  },
+  {
+    unfold cl,    
+    rw [subtype.image_preimage, cl_reg_set_inter, idempotent],
+  },
+  {
+    change y.val ∈ _,
+    change x.val ∈ _ at a,
+    change x.val ∉ _ at a_1,
+    rw set.image_insert_eq at *,
+    exact exchange a a_1,
+  },
+  {
+    change x.val ∈ _ at a,
+    rcases finchar a with ⟨W,h1,h2⟩,
+    have : ↑W ≤ reg_set T,
+    {
+      refine le_trans h1 _,
+      exact subtype.image_le S,
+    },
+    rcases reg_lift_finset this with ⟨V,rfl⟩,
+    refine ⟨V,_,_⟩,
+    {
+      intros v hv,
+      rw ←subtype.preimage_image S,
+      apply h1,
+      rw finset.coe_image,
+      exact set.mem_image_of_mem ι hv,
+    },
+    {
+      rw finset.coe_image at h2,
+      exact h2,
+    }
+  },
+end
+
+@[simp]
+theorem regularity [pregeom T] : cl (∅ : set (reg T)) = ∅ := 
+begin
+  unfold cl,
+  rw set.image_empty,
+  ext, split; intro hx,
+  {
+    change x.val ∈ _ at hx,
+    have := x.2,
+    contradiction,
+  },
+  {
+    finish,
+  }
+end
+
+end reg
+
+protected def setoid [has_cl T] : setoid (reg T) := ⟨reg.rel T, reg.is_equiv⟩
+
+def geom [has_cl T] := quotient (pregeom.setoid T)
+
+namespace geom
+
+variable {T}
+
+def to_geom [has_cl T] : reg T → geom T := quotient.mk'
+
+local notation `π` := to_geom
+
+def to_geom_of_reg [has_cl T] {t : T} (h : t ∈ reg_set T) : geom T := π ⟨t,h⟩
+
+theorem eq_iff [has_cl T] {u v : reg T} : π u = π v ↔ cls u = cls v := by simpa [to_geom]
+
+theorem eq_iff' [pregeom T] {u v : reg T} : π u = π v ↔ u ∈ cls v :=
+begin
+  rw eq_iff,
+  split,
+  {
+    intro h, rw ←h, exact mem_cls,
+  },
+  {
+    intro h1, ext, split,
+    {
+      intro h2,
+      unfold cls at h1,
+      rw ←cls_le at h1,
+      exact h1 h2,
+    },
+    {
+      intro h2,
+      replace h1 := exchange_cls h1 _,
+      {
+        unfold cls at h1,
+        rw ←cls_le at h1,
+        exact h1 h2,
+      },
+      {
+        rw reg.regularity,
+        tauto,
+      }
+    }
+  }
+end
+
+theorem cls_le_pullback_of_mem [pregeom T] {t : reg T} {S : set (geom T) }: π t ∈ S ↔ cls t ≤ π ⁻¹' S :=
+begin
+  split; intro h,
+  {
+    intros u hu,
+    change _ ∈ cls _ at hu,
+    rw ←eq_iff' at hu,
+    rwa ←hu at h,
+  },
+  {
+    suffices : t ∈ π ⁻¹' S, by exact this,
+    apply h,
+    exact mem_cls,
+  }
+end
+
+lemma mem_cl_of_mem_mk_eq_mk [pregeom T] {x y : reg T} {S : set (reg T)} : x ∈ cl S → π x = π y → y ∈ cl S := 
+begin
+  intros hx h,
+  suffices : cls y ≤ cl S, by exact this mem_cls,
+  rw eq_iff at h,
+  rw ←h,
+  rw ←cls_le_of_mem,
+  assumption,
+end
+
+lemma mem_cl_of_mk_eq_mk [pregeom T] {a b : reg T} {S : set (reg T)} : a ∈ S → π b = π a → b ∈ cl S :=
+begin
+  intros ha h,
+  rw eq_iff' at h,
+  replace ha : ({a} : set (reg T)) ≤ S, 
+  {
+    rintros b ⟨rfl⟩,
+    assumption,
+  },
+  apply monotone ha,
+  assumption,
+end
+
+instance has_cl_instance [has_cl T] : has_cl (geom T) := 
+⟨ λ S, π '' (cl (π ⁻¹' S)) ⟩
+
+variable [pregeom T]
+
+lemma pi_mem_cl_iff_mem_cl_preimage {t : reg T} {S : set (geom T)} : 
+  t ∈ cl (π ⁻¹' S) ↔ π t ∈ cl S :=
+begin
+  split; intro h,
+  {
+    exact ⟨t,h,rfl⟩,
+  },
+  {
+    rcases h with ⟨u,h,hu⟩,
+    exact mem_cl_of_mem_mk_eq_mk h hu,
+  }
+end
+
+lemma cl_pullback_cl_eq_cl_pullback {S : set (geom T)} : cl (π ⁻¹' cl S) = cl (π ⁻¹' S) := 
+begin
+  ext, split; intro hx,
+  {
+    rw ←idempotent,
+    refine monotone _ hx,
+    intros y hy,
+    change π y ∈ _ at hy,
+    rwa ←pi_mem_cl_iff_mem_cl_preimage at hy,
+  },
+  {
+    -- This is the same as the inclusive proof in the pregeom instance.
+    -- Should be made into a seaprate lemma to avoid repetition
+    refine monotone _ hx,
+    refine set.preimage_mono _,
+    intros s hs,
+    rcases quot.exists_rep s with ⟨t,ht⟩,
+    change π _ = _ at ht,
+    refine ⟨t,_,ht⟩,
+    suffices : cls t ≤ π ⁻¹' S,
+    {
+      apply inclusive,
+      apply this,
+      apply mem_cls,
+    },
+    intros u hu,
+    change π u ∈ S,
+    rw ←eq_iff' at hu,
+    rwa [hu,ht],
+  }
+end
+
+@[simp]
+lemma pullback_insert {t : reg T} {S : set (geom T)} : π ⁻¹' insert (π t) S = cls t ∪ π ⁻¹' S := 
+begin
+  ext, split; intro hx,
+  {
+    change π x ∈ _ at hx,
+    cases hx,
+    {
+      left,
+      rwa eq_iff' at hx,
+    },
+    {
+      right,
+      exact hx,
+    }
+  },
+  {
+    change π x ∈ _,
+    cases hx,
+    {
+      left,
+      rwa eq_iff',
+    },
+    {
+      right,
+      exact hx,
+    }
+  }
+end
+
+lemma cl_preimage_insert {t : reg T} {S : set (geom T)} : cl (π ⁻¹' insert (π t) S) = cl (insert t (π ⁻¹' S)) := 
+begin
+  rw pullback_insert,
+  unfold cls,
+  rw cl_cl_union,
+  rw set.singleton_union,
+end
+
+instance pregeom_instance : pregeom (geom T) :=
+begin
+  split; intros,
+  {
+    intros s hs,
+    rcases quot.exists_rep s with ⟨t,ht⟩,
+    change π _ = _ at ht,
+    refine ⟨t,_,ht⟩,
+    suffices : cls t ≤ π ⁻¹' S, 
+    {
+      apply inclusive,
+      apply this,
+      apply mem_cls,
+    },
+    intros u hu,
+    change π u ∈ S,
+    rw ←eq_iff' at hu,
+    rwa [hu, ht],
+  },
+  {
+    intros a ha,
+    rcases quot.exists_rep a with ⟨t,ht⟩,
+    change π _ = _ at ht,
+    refine ⟨t,_,ht⟩,
+    have : π ⁻¹' A ≤ π ⁻¹' B, 
+    {
+      change _ ⊆ _,
+      apply set.preimage_mono,
+      assumption,
+    },
+    apply monotone this,
+    rw ←ht at ha,
+    rwa pi_mem_cl_iff_mem_cl_preimage,
+  },
+  {
+    ext, split; intro hx,
+    {
+      rcases hx with ⟨y,hy,rfl⟩,
+      rw cl_pullback_cl_eq_cl_pullback at hy,
+      exact ⟨y,hy,rfl⟩,
+    },
+    {
+      rcases hx with ⟨y,hy,rfl⟩,
+      rw ←cl_pullback_cl_eq_cl_pullback at hy,
+      exact ⟨y,hy,rfl⟩,
+    }
+  },
+  {
+    rcases a with ⟨a,ha,rfl⟩,
+    rcases quot.exists_rep y with ⟨t,rfl⟩,
+    change _ ∈ cl ( π ⁻¹' insert (π _) _) at ha,
+    change π t ∈ _,
+    rw cl_preimage_insert at ha,
+    have : a ∉ cl (π ⁻¹' S), 
+    {
+      intro contra,
+      rw pi_mem_cl_iff_mem_cl_preimage at contra,
+      contradiction,
+    },
+    replace this := exchange ha this,
+    rw [←pi_mem_cl_iff_mem_cl_preimage, cl_preimage_insert],
+    assumption,
+  },
+  {
+    rcases a with ⟨y,hy,rfl⟩,
+    rcases finchar hy with ⟨W,hW1,hW2⟩,
+    refine ⟨finset.image π W,_,_⟩,
+    {
+      intros w hw,
+      rw finset.coe_image at hw,
+      rcases hw with ⟨u,hu,rfl⟩,
+      replace hu := hW1 hu,
+      exact hu,
+    },
+    {
+      rw finset.coe_image,
+      rw ←pi_mem_cl_iff_mem_cl_preimage, 
+      refine monotone _ hW2,
+      intros w hw,
+      change π w ∈ _,
+      exact set.mem_image_of_mem π hw,
+    }
+  },
+end
+
+lemma mem_cls_geom [pregeom T] {x y : geom T} : x ∈ cls y → x = y := 
+begin
+  intro hx,
+  rcases hx with ⟨z,hz,rfl⟩,
+  rcases quot.exists_rep y with ⟨w,hw,rfl⟩,
+  rw set.singleton_def at hz,
+  change _ ∈ cl ( π ⁻¹' (insert (π w) _) ) at hz,
+  rw pullback_insert at hz,
+  change π z = π _,
+  unfold cls at hz,
+  rw pregeom.cl_cl_union at hz,
+  simp only [insert_emptyc_eq, set.singleton_union, set.preimage_empty] at hz,
+  change z ∈ cls w at hz,
+  rwa eq_iff',
+end
+
+instance geom_instance : geometry (geom T) := 
+begin
+  split,
+  {
+    intro x,
+    ext y, split; intro hy,
+    {
+      change y = x,
+      apply mem_cls_geom,
+      assumption,
+    },
+    {
+      change y = x at hy,
+      rw hy,
+      exact mem_cls,
+    }
+  },
+  {
+    change π '' cl (∅ : set (reg T)) = _,
+    rw reg.regularity,
+    finish,
+  }
+end
+
+end geom
+
+end pregeom
