src/subtype/helpers.lean
@@ -1,0 +1,49 @@
+import data.set
+
+variables {T : Type*} {S : set T}
+
+namespace subtype
+
+local notation `ι` := val
+
+@[simp]
+lemma image_preimage (A : set T) : ι '' (ι ⁻¹' A : set (subtype S)) = S ∩ A :=
+begin
+  ext,
+  split,
+  {
+    intro h,
+    rcases h with ⟨y,h,rfl⟩,
+    exact ⟨y.2,h⟩
+  },
+  {
+    intro h,
+    exact ⟨⟨x,h.1⟩,h.2,by refl⟩
+  }
+end
+
+@[simp]
+lemma preimage_image (A : set (subtype S)) : ι ⁻¹' (ι '' A) = A := 
+begin
+  ext, split,
+  {
+    intro h,
+    cases x with x hx,
+    change x ∈ _ at h,
+    rcases h with ⟨y,h,rfl⟩,
+    finish,
+  },
+  {
+    intro h,
+    change x.val ∈ ι '' A,
+    exact set.mem_image_of_mem ι h,
+  }
+end
+
+lemma image_le (A : set (subtype S)) : ι '' A ≤ S := 
+begin
+  rintros a ⟨b,hb,rfl⟩,
+  exact b.2
+end
+
+end subtype
